partition refinement: WIP, some issues...

src/SlabsAlloc.fst
@@ -28,7 +28,6 @@ open SteelStarSeqUtils
 open FStar.Mul
 open SlabsCommon
 
-#reset-options "--ifuel 1 --fuel 1"
 
 #push-options "--z3rlimit 50"
 inline_for_extraction noextract
@@ -154,6 +153,8 @@ let md_region_mon_split
 
 open SteelVRefineDep
 
+#restart-solver
+
 #push-options "--z3rlimit 100 --compat_pre_typed_indexed_effects"
 inline_for_extraction noextract
 let allocate_slab_aux_1_partial
@@ -191,13 +192,15 @@ let allocate_slab_aux_1_partial
       (left_vprop size_class slab_region md_bm_region md_region r1 r2 r3)
   )
   (requires fun h0 ->
+    let gs0 = AL.v_arraylist pred1 pred2 pred3 (A.split_l md_region (u32_to_sz md_count_v)) (US.v idx1) (US.v idx2) (US.v idx3) h0 in
     U32.v md_count_v <> AL.null /\
     sel md_count h0 == md_count_v /\
     sel r1 h0 == idx1 /\
     sel r2 h0 == idx2 /\
     sel r3 h0 == idx3 /\
     idx1 <> AL.null_ptr /\
-    ALG.dataify (AL.v_arraylist pred1 pred2 pred3 (A.split_l md_region (u32_to_sz md_count_v)) (US.v idx1) (US.v idx2) (US.v idx3) h0) `Seq.equal` Ghost.reveal md_region_lv
+    ALG.dataify gs0 `Seq.equal` G.reveal md_region_lv /\
+    ALG.partition #AL.status gs0 (US.v idx1) (US.v idx2) (US.v idx3)
   )
   (ensures fun _ _ h1 ->
     let blob1
@@ -208,18 +211,23 @@ let allocate_slab_aux_1_partial
     ) in
     md_count_v == dfst blob1)
   =
+  (**) let _ = gget (AL.varraylist pred1 pred2 pred3
+    (A.split_l md_region (u32_to_sz md_count_v))
+    (US.v idx1) (US.v idx2) (US.v idx3)) in
   (**) ALG.lemma_head_not_null_mem pred1 pred2 pred3
     (A.split_l md_region (u32_to_sz md_count_v))
     idx1 idx2 idx3;
-  // required for selector equality propagation
-  (**) let _ = gget (AL.varraylist pred1 pred2 pred3 (A.split_l md_region (u32_to_sz md_count_v)) (US.v idx1) (US.v idx2) (US.v idx3)) in
-
   let idx1' = AL.remove1 #pred1 #pred2 #pred3
     (A.split_l md_region (u32_to_sz md_count_v))
     idx1 (Ghost.hide (US.v idx2)) (Ghost.hide (US.v idx3)) idx1 in
   AL.insert2 #pred1 #pred2 #pred3
     (A.split_l md_region (u32_to_sz md_count_v))
     idx2 (Ghost.hide (US.v idx1')) (Ghost.hide (US.v idx3)) idx1 1ul;
+  (**) let gs0 = gget (AL.varraylist pred1 pred2 pred3
+    (A.split_l md_region (u32_to_sz md_count_v))
+    (US.v idx1') (US.v idx1) (US.v idx3)) in
+  assume (ALG.partition #AL.status gs0 (US.v idx1') (US.v idx1) (US.v idx3));
+
   write r1 idx1';
   write r2 idx1;
 
@@ -263,13 +271,15 @@ let allocate_slab_aux_1_full
       (left_vprop size_class slab_region md_bm_region md_region r1 r2 r3)
   )
   (requires fun h0 ->
+    let gs0 = AL.v_arraylist pred1 pred2 pred3 (A.split_l md_region (u32_to_sz md_count_v)) (US.v idx1) (US.v idx2) (US.v idx3) h0 in
     U32.v md_count_v <> AL.null /\
     sel md_count h0 == md_count_v /\
     sel r1 h0 == idx1 /\
     sel r2 h0 == idx2 /\
     sel r3 h0 == idx3 /\
     idx1 <> AL.null_ptr /\
-    ALG.dataify (AL.v_arraylist pred1 pred2 pred3 (A.split_l md_region (u32_to_sz md_count_v)) (US.v idx1) (US.v idx2) (US.v idx3) h0) `Seq.equal` Ghost.reveal md_region_lv
+    ALG.dataify gs0 `Seq.equal` G.reveal md_region_lv /\
+    ALG.partition #AL.status gs0 (US.v idx1) (US.v idx2) (US.v idx3)
   )
   (ensures fun _ _ h1 ->
     let blob1
@@ -292,6 +302,10 @@ let allocate_slab_aux_1_full
   AL.insert3 #pred1 #pred2 #pred3
     (A.split_l md_region (u32_to_sz md_count_v))
     idx3 (Ghost.hide (US.v idx1')) (Ghost.hide (US.v idx2)) idx1 2ul;
+  (**) let gs0 = gget (AL.varraylist pred1 pred2 pred3
+    (A.split_l md_region (u32_to_sz md_count_v))
+    (US.v idx1') (US.v idx2) (US.v idx1)) in
+  assume (ALG.partition #AL.status gs0 (US.v idx1') (US.v idx2) (US.v idx1));
   write r1 idx1';
   write r3 idx1;
 
@@ -335,13 +349,15 @@ let allocate_slab_aux_1
       (left_vprop size_class slab_region md_bm_region md_region r1 r2 r3)
   )
   (requires fun h0 ->
+    let gs0 = AL.v_arraylist pred1 pred2 pred3 (A.split_l md_region (u32_to_sz md_count_v)) (US.v idx1) (US.v idx2) (US.v idx3) h0 in
     U32.v md_count_v <> AL.null /\
     sel md_count h0 == md_count_v /\
     sel r1 h0 == idx1 /\
     sel r2 h0 == idx2 /\
     sel r3 h0 == idx3 /\
     idx1 <> AL.null_ptr /\
-    ALG.dataify (AL.v_arraylist pred1 pred2 pred3 (A.split_l md_region (u32_to_sz md_count_v)) (US.v idx1) (US.v idx2) (US.v idx3) h0) `Seq.equal` Ghost.reveal md_region_lv
+    ALG.dataify gs0 `Seq.equal` G.reveal md_region_lv /\
+    ALG.partition #AL.status gs0 (US.v idx1) (US.v idx2) (US.v idx3)
   )
   (ensures fun _ _ h1 ->
     let blob1
@@ -405,6 +421,7 @@ let allocate_slab_aux_1
 #pop-options
 
 #restart-solver
+
 #push-options "--z3rlimit 75 --compat_pre_typed_indexed_effects"
 inline_for_extraction noextract
 let allocate_slab_aux_2_full
@@ -442,13 +459,15 @@ let allocate_slab_aux_2_full
       (left_vprop size_class slab_region md_bm_region md_region r1 r2 r3)
   )
   (requires fun h0 ->
+    let gs0 = AL.v_arraylist pred1 pred2 pred3 (A.split_l md_region (u32_to_sz md_count_v)) (US.v idx1) (US.v idx2) (US.v idx3) h0 in
     U32.v md_count_v <> AL.null /\
     sel md_count h0 == md_count_v /\
     sel r1 h0 == idx1 /\
     sel r2 h0 == idx2 /\
     sel r3 h0 == idx3 /\
     idx2 <> AL.null_ptr /\
-    ALG.dataify (AL.v_arraylist pred1 pred2 pred3 (A.split_l md_region (u32_to_sz md_count_v)) (US.v idx1) (US.v idx2) (US.v idx3) h0) `Seq.equal` Ghost.reveal md_region_lv
+    ALG.dataify gs0 `Seq.equal` G.reveal md_region_lv /\
+    ALG.partition #AL.status gs0 (US.v idx1) (US.v idx2) (US.v idx3)
   )
   (ensures fun _ _ h1 ->
     let blob1
@@ -471,6 +490,10 @@ let allocate_slab_aux_2_full
   AL.insert3 #pred1 #pred2 #pred3
     (A.split_l md_region (u32_to_sz md_count_v))
     idx3 (Ghost.hide (US.v idx1)) (Ghost.hide (US.v idx2')) idx2 2ul;
+  (**) let gs0 = gget (AL.varraylist pred1 pred2 pred3
+    (A.split_l md_region (u32_to_sz md_count_v))
+    (US.v idx1) (US.v idx2') (US.v idx2)) in
+  assume (ALG.partition #AL.status gs0 (US.v idx1) (US.v idx2') (US.v idx2));
   write r2 idx2';
   write r3 idx2;
 
@@ -514,13 +537,15 @@ let allocate_slab_aux_2_partial
       (left_vprop size_class slab_region md_bm_region md_region r1 r2 r3)
   )
   (requires fun h0 ->
+    let gs0 = AL.v_arraylist pred1 pred2 pred3 (A.split_l md_region (u32_to_sz md_count_v)) (US.v idx1) (US.v idx2) (US.v idx3) h0 in
     U32.v md_count_v <> AL.null /\
     sel md_count h0 == md_count_v /\
     sel r1 h0 == idx1 /\
     sel r2 h0 == idx2 /\
     sel r3 h0 == idx3 /\
     idx2 <> AL.null_ptr /\
-    ALG.dataify (AL.v_arraylist pred1 pred2 pred3 (A.split_l md_region (u32_to_sz md_count_v)) (US.v idx1) (US.v idx2) (US.v idx3) h0) `Seq.equal` Ghost.reveal md_region_lv
+    ALG.dataify gs0 `Seq.equal` G.reveal md_region_lv /\
+    ALG.partition #AL.status gs0 (US.v idx1) (US.v idx2) (US.v idx3)
   )
   (ensures fun _ _ h1 ->
     let blob1
@@ -570,14 +595,15 @@ let allocate_slab_aux_2
       (left_vprop size_class slab_region md_bm_region md_region r1 r2 r3)
   )
   (requires fun h0 ->
+    let gs0 = AL.v_arraylist pred1 pred2 pred3 (A.split_l md_region (u32_to_sz md_count_v)) (US.v idx1) (US.v idx2) (US.v idx3) h0 in
     U32.v md_count_v <> AL.null /\
     sel md_count h0 == md_count_v /\
     sel r1 h0 == idx1 /\
     sel r2 h0 == idx2 /\
     sel r3 h0 == idx3 /\
     idx2 <> AL.null_ptr /\
-    ALG.dataify (AL.v_arraylist pred1 pred2 pred3 (A.split_l md_region (u32_to_sz md_count_v)) (US.v idx1) (US.v idx2) (US.v idx3) h0) `Seq.equal` Ghost.reveal md_region_lv
-
+    ALG.dataify gs0 `Seq.equal` G.reveal md_region_lv /\
+    ALG.partition #AL.status gs0 (US.v idx1) (US.v idx2) (US.v idx3)
   )
   (ensures fun _ _ h1 ->
     let blob1
@@ -1328,6 +1354,7 @@ let allocate_slab
   let idx1_ = read r1 in
   let idx2_ = read r2 in
   let idx3_ = read r3 in
+  sladmit ();
 
   change_slprop_rel
     (AL.varraylist pred1 pred2 pred3
